WIP: track the (partial) codomain of a TotalMapping

SSA/Experimental/IntrinsicAsymptotics/Mapping.lean
@@ -1,6 +1,8 @@
 import SSA.Experimental.IntrinsicAsymptotics.Context
 
 
+/-! ### Mapping -/
+
 def Mapping.Pair (Γ Δ : Ctxt) := Σ t, Γ.Var t × Δ.Var t
 
 /-- `Mapping Γ Δ` is an incrementally built a mapping from variables in `Γ` to variables in `Δ` -/
@@ -57,46 +59,113 @@ def Mapping.lookup : Mapping Γ Δ → (t : Ty) → Γ.Var t → Option (Δ.Var 
         lookup map t' v'
 
 
-structure TotalMapping (Γ Δ : Ctxt) (V : Γ.VarSet) where
-  inner : Mapping Γ Δ
-  -- isTotal : ∀ t, ∀ v ∈ expr.vars, (inner.lookup t v).isSome
-  isTotal : ∀ t, ∀ v ∈ V t, (inner.lookup t v).isSome
 
-def TotalMapping.empty : TotalMapping Γ Δ ∅ :=
-  ⟨[], by intros; contradiction⟩
+
+/-! ### Total Mapping -/
+
+/--
+  A `TotalMapping Γ Δ V` is just a `Mapping`, with extra knowledge about the variables that are
+  alreaady assigned.
+  That is, `constraints` is a list of pairs `(V, W)` of variables in the domain and codomain, 
+  respectively, such that each variable `v ∈ V` is assigned to a variable `w ∈ W` in the 
+  corresponding set.
+  These constraints form a stack. `insert v w` adds `v` to the top-most set `V`, and require that 
+  `w` is already present in the top-most `W`.
+-/
+structure TotalMapping (Γ Δ : Ctxt) (constraints : List (Γ.VarSet × Δ.VarSet)) where
+  inner : Mapping Γ Δ
+  isTotal : ∀ V W, (V, W) ∈ constraints → 
+    ∀ t, ∀ v ∈ V t, ∃ w ∈ W t, inner.lookup t v = some w
+
+/-- An empty map, with `W` as the top-most constraint on the codomain -/
+def TotalMapping.empty (W : Δ.VarSet) : TotalMapping Γ Δ [(∅, W)] :=
+  ⟨[], by intro V W mem h v v_mem; simp at mem; simp[mem] at v_mem; contradiction⟩
+
+
+/-- Adds a new top-most constraint, without changing anything about the underlying map -/
+def TotalMapping.newConstraint (W : Δ.VarSet) :
+    TotalMapping Γ Δ constraints → TotalMapping Γ Δ ((∅, W) :: constraints)
+  | ⟨map, isTotal⟩ => ⟨map, by
+      intro V W mem
+      cases mem
+      next => intros; contradiction
+      next mem_tl => apply isTotal V W mem_tl
+    ⟩ 
+
+/-- Combine the two top-most constraints, by taking the union of the respective sets -/
+def TotalMapping.popConstraint :
+    TotalMapping Γ Δ ((V₁, W₁) :: (V₂, W₂) :: constraints) 
+    → TotalMapping Γ Δ ((V₁ ∪ V₂, W₁ ∪ W₂) :: constraints)
+  | ⟨map, isTotal⟩ => ⟨map, by
+      intro V W mem
+      cases mem
+      case head =>
+        intro t v h_v
+        cases h_v
+        case inl h_v =>
+          rcases isTotal V₁ W₁ (List.Mem.head _) t v h_v with ⟨w, mem_w, h_lookup⟩
+          refine ⟨w, Or.inl mem_w, h_lookup⟩ 
+        case inr h_v =>
+          rcases isTotal V₂ W₂ (List.Mem.tail _ <| List.Mem.head _) t v h_v with ⟨w, mem_w, h_lookup⟩
+          refine ⟨w, Or.inr mem_w, h_lookup⟩ 
+      case tail mem =>
+        apply isTotal V W (List.Mem.tail _ <| List.Mem.tail _ mem)
+    ⟩
+
+
+
+/-- If mapping succeeds, then `v` and `w` must have the same type -/
+theorem Mapping.type_eq_of_insert_isSome {map : Mapping Γ Δ} {v : Γ.Var t₁} {w : Δ.Var t₂} :
+    map.insert v w = some mapI → t₁ = t₂ := by
+  simp only [insert, Option.isSome]
+  split_ifs
+  . intro; assumption
+  . exact False.elim
 
 
 /-- After `insert`ing a variable mapping for `v`, `lookup` is guaranteed to be defined on `v` -/
 theorem Mapping.lookup_insert_same (map mapInsert : Mapping Γ Δ) {v : Γ.Var t₁} (w : Δ.Var t₂)
-    (h : map.insert v w = some mapInsert) :
-    (mapInsert.lookup _ v).isSome := by
-  unfold insert at h
-  unfold Option.isSome
-  split_ifs at h
+    (h_insert : map.insert v w = some mapInsert) :
+    (mapInsert.lookup _ v) = some (cast (by rw[type_eq_of_insert_isSome h_insert]) w) := by
+  cases (type_eq_of_insert_isSome h_insert)
+  simp only [insert, cast_eq, dite_eq_ite, ite_true] at h_insert 
+  simp only [cast_eq]  
+
   induction map generalizing mapInsert
   next =>
-    simp only [insert.go, Option.some.injEq] at h 
-    simp [←h, Option.isSome, lookup]
+    simp only [insert.go, Option.some.injEq] at h_insert
+    simp [←h_insert, Option.isSome, lookup]
   next m map ih =>
-    simp only [insert.go, Prod.mk.eta, Sigma.eta] at h    
-    split_ifs at h <;> simp at h
-    . cases h
+    simp only [insert.go, Prod.mk.eta, Sigma.eta] at h_insert
+    split_ifs at h_insert <;> simp at h_insert
+    next h_v h_w =>
+      cases h_insert
       simp only [lookup]
       split_ifs
+      
+      rcases m with ⟨tm, ⟨v', v'_prop⟩, ⟨w', w'_prop⟩⟩
+      rcases w with ⟨w, w_prop⟩
+      cases h_w
+      rw[w'_prop, Option.some_inj] at w_prop
+      cases w_prop
+
       rfl
-    . rcases h with ⟨tl, ⟨h₁, ⟨⟩⟩⟩
+    next => 
+      rcases h_insert with ⟨tl, ⟨h₁, ⟨⟩⟩⟩
       simp[lookup]
       split_ifs
+      simp at ih
       apply ih _ h₁
+
+      
 
 /-- If `insert` succeeds, it only add new mappings.
     Thus if `lookup` is defined previous to an insert, then lookup will remain defined afterwards
  -/
 theorem Mapping.lookup_insert_preserve (map mapInsert : Mapping Γ Δ) {v : Γ.Var t₁} (w : Δ.Var t₂)
-    {v' : Γ.Var t₃} (h : map.insert v w = some mapInsert) :
-    (map.lookup t₃ v').isSome → (mapInsert.lookup t₃ v').isSome := by
+    {v' : Γ.Var t₃} (h : map.insert v w = some mapInsert) (z) :
+    (map.lookup t₃ v') = some z → (mapInsert.lookup t₃ v') = some z := by
   unfold insert at h
-  unfold Option.isSome
   split_ifs at h
   induction map generalizing mapInsert
   next =>
@@ -116,42 +185,79 @@ theorem Mapping.lookup_insert_preserve (map mapInsert : Mapping Γ Δ) {v : Γ.V
 /--
   By inserting into a total mapping, we expand the set of variables that it is defined on
 -/
-def TotalMapping.insert (map : TotalMapping Γ Δ V) (v : Γ.Var t₁) (w : Δ.Var t₂) : 
-    Option (TotalMapping Γ Δ (V ∪ {⟨_, v⟩})) := 
-  match hm : map.inner.insert v w with
+def TotalMapping.insert (map : TotalMapping Γ Δ ((V,W) :: tl)) (v : Γ.Var t₁) (w : Δ.Var t₂) 
+    (h_w : w ∈ W _) : 
+    Option (TotalMapping Γ Δ ((V ∪ {⟨_, v⟩}, W) :: tl)) := 
+  match h_insert : map.inner.insert v w with
     | .some mapI => some {
         inner := mapI
         isTotal := by 
-          intro t' v' h
-          rcases map with ⟨map, isTotal⟩          
-          dsimp[Membership.mem, Set.Mem, Union.union, Set.union, setOf] at h
-          cases h
-          next h => 
-            apply Mapping.lookup_insert_preserve map mapI w hm
-            apply isTotal _ _ h
-          next h =>
-            apply Mapping.lookup_insert_same map mapI w
-            simp at h
-            cases (Ctxt.Var.type_eq_of_index_eq h)
-            rcases v with ⟨v, hv⟩
-            rcases v' with ⟨v', hv'⟩
-            cases h
-            apply hm
+          intro V W h_mem t' v' h_v'
+          cases (Mapping.type_eq_of_insert_isSome h_insert)
+          rcases map with ⟨map, isTotal⟩
+          cases h_mem
+          next =>
+            specialize isTotal V W (List.Mem.head ..) t' v'
+            dsimp[Membership.mem, Set.Mem, Union.union, Set.union, setOf] at h_v'
+            cases h_v'
+            next h_v' => 
+              rcases isTotal h_v' with ⟨w', h_w', h_lookup⟩
+              refine ⟨w', h_w', ?_⟩
+              apply Mapping.lookup_insert_preserve 
+              <;> assumption              
+            next h_v' =>
+              rcases v with ⟨v, prop_v⟩
+              rcases v' with ⟨v', prop_v'⟩
+              cases h_v'
+              rw[prop_v', Option.some_inj] at prop_v
+              cases prop_v
+              
+              rw [Mapping.lookup_insert_same map mapI w h_insert, cast_eq]
+              exact ⟨w, h_w, rfl⟩
+            
+          next h_mem =>
+            rcases isTotal _ _ (List.Mem.tail _ h_mem) t' v' h_v' with ⟨w', h_w', h_insert⟩
+            refine ⟨w', h_w', ?_⟩
+            apply Mapping.lookup_insert_preserve 
+            <;> assumption         
       }
     | .none => none
 
 
+
+
+
 /-- Change the set of variables that a total mapping is known to be defined on  -/
-def TotalMapping.coerceDomain {Γ : Ctxt} {V V' : Γ.VarSet} (h : V = V') : 
-    TotalMapping Γ Δ V → TotalMapping Γ Δ V' 
-  | ⟨inner, isTotal⟩ => ⟨inner, by simp_all⟩
+def TotalMapping.coerceConstraint {Γ : Ctxt} {V V' : Γ.VarSet} {W W' : Δ.VarSet} {cs}
+    (hV : V = V') (hW : W = W') : 
+    TotalMapping Γ Δ ((V, W) :: cs) → TotalMapping Γ Δ ((V', W') :: cs)
+  | ⟨inner, isTotal⟩ => ⟨inner, by cases hV; cases hW; exact isTotal⟩
+
+
+/-- A specialization of the `isTotal` property to just the constraint at the top of the stack -/
+theorem TotalMapping.isTotal_head (map : TotalMapping Γ Δ ((V, W) :: cs)) :
+    ∀ v ∈ V t, ∃ w ∈ W t, map.inner.lookup t v = some w :=
+  map.isTotal V W (List.Mem.head _) t
 
 /-- `lookup` a variable that is known to occur in a total map -/
-def TotalMapping.lookupMem (map : TotalMapping Γ Δ V) (t : Ty) (v : Γ.Var t) : v ∈ V t → Δ.Var t :=
-  (map.inner.lookup t v).get ∘ map.isTotal t v
+def TotalMapping.lookupMem (map : TotalMapping Γ Δ ((V, W) :: cs)) (t : Ty) (v : Γ.Var t) : 
+    v ∈ V t → {w : Δ.Var t // w ∈ W t} :=
+  fun h_v => ⟨
+    (map.inner.lookup t v).get (by
+      rcases (map.isTotal_head v h_v) with ⟨w, _, eq⟩
+      rw[Option.isSome, eq]
+    ),
+    by 
+      rcases (map.isTotal_head v h_v) with ⟨w, h_w, eq⟩
+      have : Option.isSome (Mapping.lookup map.inner t v) := by
+        simp_all
+      rw [Option.get_of_mem this ?_]
+      . assumption
+      . rw[eq]; rfl
+  ⟩
 
 /-- If the set of known-assigned variables is complete w.r.t. its context, then we can return a 
     total change of variables function -/
-def TotalMapping.lookup (map : TotalMapping Γ Δ V) (h : V.IsComplete) (t : Ty) (v : Γ.Var t) :
+def TotalMapping.lookup (map : TotalMapping Γ Δ ((V, W) :: cs)) (h : V.IsComplete) (t : Ty) (v : Γ.Var t) :
     Δ.Var t :=
   map.lookupMem t v (h t v)
